Refactor trace equivalence proofs

theories/Equiv/TraceEquiv.v
@@ -1,78 +1,12 @@
 Require Import List.
-Require Export Util Var Val Exp Env Map CSet AutoIndTac IL AllInRel.
-Require Export SmallStepRelations StateType NonParametricBiSim Sim.
+Require Import Util Var Val Exp Env Map CSet AutoIndTac IL AllInRel.
+Require Import SmallStepRelations StateType NonParametricBiSim.
+Require Import Divergence StateTypeProperties.
 
 Set Implicit Arguments.
 Unset Printing Records.
 
-(** * Divergence *)
-
-CoInductive diverges S `{StateType S} : S -> Prop :=
-| DivergesI σ σ'
-  : step σ EvtTau σ'
-    -> diverges σ'
-    -> diverges σ.
-
-Lemma diverges_reduction_closed S `{StateType S} (σ σ':S)
-: diverges σ -> star2 step σ nil σ'  -> diverges σ'.
-Proof.
-  intros. general induction H1; eauto using diverges.
-  invt diverges; relsimpl. eauto.
-Qed.
-
-Lemma diverges_never_activated S `{StateType S} (σ:S)
-: activated σ -> diverges σ -> False.
-Proof.
-  intros. invt diverges; relsimpl.
-Qed.
-
-Lemma diverges_never_terminates S `{StateType S} (σ:S)
-: normal2 step σ -> diverges σ -> False.
-Proof.
-  intros. invt diverges; relsimpl.
-Qed.
-
-(** ** Bisimilarity preserves silent divergence *)
-
-Lemma bisim_sound_diverges S `{StateType S} S' `{StateType S'} (σ:S) (σ':S')
-: bisim σ σ' -> diverges σ -> diverges σ'.
-Proof.
-  revert σ σ'. cofix COH; intros.
-  inv H1.
-  - eapply plus2_destr_nil in H4. dcr.
-    econstructor. eauto.
-    eapply COH; eauto.
-    eapply simp_bisim.
-    eapply sim_reduction_closed.
-    eapply bisim_simp. eapply H1. econstructor.
-    eapply (star2_step EvtTau); eauto. econstructor.
-  - eapply diverges_reduction_closed in H3.
-    + exfalso. eapply (diverges_never_activated H5); eauto.
-    + eapply H2.
-  - eapply diverges_reduction_closed in H4.
-    + exfalso. eapply (diverges_never_terminates H6); eauto.
-    + eapply H2.
-Qed.
-
-(** ** Silently diverging programs are bisimlar *)
-
-Lemma bisim_complete_diverges S `{StateType S} S' `{StateType S'} (σ:S) (σ':S')
-: diverges σ -> diverges σ' -> bisim σ σ'.
-Proof.
-  revert σ σ'. cofix COH; intros.
-  inv H1; inv H2.
-  econstructor. econstructor; eauto. econstructor; eauto.
-  eapply COH; eauto.
-Qed.
-
-
 (** * Prefix Trace Equivalence (partial traces) **)
-
-(** A prefix is a list of [extevent] *)
-
-Inductive extevent :=
-  | EEvtExtern (evt:event)
-  | EEvtTerminate (res:option val).
 
 (** A relation that assigns prefixes to states *)
 
@@ -123,76 +57,22 @@ Qed.
 
 (** ** Bisimilarity is sound for prefix inclusion *)
 
-Lemma bisim_terminate {S1} `{StateType S1} (σ1 σ1':S1)
-      {S2} `{StateType S2} (σ2:S2)
-: star2 step σ1 nil σ1'
-  -> normal2 step σ1'
-  -> sim bot3 Bisim σ1 σ2
-  -> exists σ2', star2 step σ2 nil σ2' /\ normal2 step σ2' /\ result σ1' = result σ2'.
-Proof.
-  intros. general induction H1.
-  - pinversion H3; subst.
-    + exfalso. eapply H2. inv H1; do 2 eexists; eauto.
-    + exfalso. eapply star2_normal in H1; eauto. subst.
-      eapply (activated_normal _ H5); eauto.
-    + eapply star2_normal in H4; eauto; subst.
-      eexists; split; eauto.
-  - destruct y; isabsurd. simpl.
-    eapply IHstar2; eauto.
-    eapply sim_reduction_closed_1; eauto using star2, star2_silent.
-Qed.
-
-
-Lemma bisim_activated {S1} `{StateType S1} (σ1:S1)
-      {S2} `{StateType S2} (σ2:S2)
-: activated σ1
-  -> sim bot3 Bisim σ1 σ2
-  -> exists σ2', star2 step σ2 nil σ2' /\ activated σ2' /\
-           ( forall (evt : event) (σ1'' : S1),
-               step σ1 evt σ1'' ->
-               exists σ2'' : S2,
-                 step σ2' evt σ2'' /\
-                 (sim bot3 Bisim σ1'' σ2''))
-           /\
-           ( forall (evt : event) (σ2'' : S2),
-               step σ2' evt σ2'' ->
-               exists σ1' : S1,
-                 step σ1 evt σ1' /\
-                 (sim bot3 Bisim σ1' σ2'')).
-Proof.
-  intros.
-  pinversion H2; subst.
-  -  exfalso. edestruct (plus2_destr_nil H3); dcr.
-     destruct H1 as [? []].
-     exploit (step_internally_deterministic _ _ _ _ H7 H1); dcr; congruence.
-  - assert (σ1 = σ0). eapply activated_star_eq; eauto. subst σ1.
-    eexists σ3; split; eauto. split; eauto. split.
-    intros. edestruct H7; eauto; dcr. destruct H12; isabsurd.
-    eexists; split; eauto.
-    intros. edestruct H8; eauto; dcr. destruct H12; isabsurd.
-    eexists; split; eauto.
-  - exfalso. refine (activated_normal_star _ H1 _ _); eauto using star2.
-Qed.
-
 Lemma bisim_prefix' {S} `{StateType S} {S'} `{StateType S'} (sigma:S) (σ':S')
 : bisim sigma σ' -> forall L, prefix sigma L -> prefix σ' L.
 Proof.
   intros. general induction H2.
-  - eapply bisim_simp in H3.
-    eapply IHprefix; eauto.
-    eapply simp_bisim. eapply sim_reduction_closed_1; eauto.
+  - eapply IHprefix; eauto.
+    eapply bisim_reduction_closed; eauto.
     eapply (star2_step _ _ H0). eapply star2_refl.
-  - eapply bisim_simp in H4.
-    eapply sim_activated in H4; eauto.
+  - eapply bisim_activated in H4; eauto.
     destruct H4 as [? [? [? []]]].
     destruct evt.
     + eapply prefix_star2_silent; eauto.
       edestruct H6; eauto. destruct H8.
       econstructor 2. eauto. eapply H8.
       eapply IHprefix; eauto.
-      eapply simp_bisim. eapply H9.
     + exfalso; eapply (no_activated_tau_step _ H0 H1); eauto.
-  - eapply (@bisim_simp Bisim) in H4. eapply bisim_terminate in H4; eauto.
+  - eapply bisim_terminate in H4; eauto.
     destruct H4 as [? [? []]]. econstructor 3; [ | eauto | eauto]. congruence.
   - econstructor 4.
 Qed.
@@ -285,7 +165,7 @@ Proof.
 Qed.
 
 Lemma prefix_preserved' S `{StateType S} S' `{StateType S'} (σ1 σ1' σ1'':S) (σ2 σ2' σ2'':S') evt
-: (forall L : list extevent, prefix σ1 L <-> prefix σ2 L)
+: (forall L : list extevent, prefix σ1 L -> prefix σ2 L)
   -> star2 step σ1 nil σ1'
   -> activated σ1'
   -> step σ1' evt σ1''
@@ -313,10 +193,9 @@ Lemma prefix_preserved S `{StateType S} S' `{StateType S'} (σ1 σ1' σ1'':S) (�
   -> step σ2' evt σ2''
   -> forall L, prefix σ1'' L <-> prefix σ2'' L.
 Proof.
-  split; intros.
-  eapply (prefix_preserved' _ _ H1); eauto.
-  symmetry in H1.
-  eapply (prefix_preserved' _ _ H1); eauto.
+  split.
+  - eapply prefix_preserved'; try eassumption. firstorder.
+  - eapply prefix_preserved'; try eassumption. firstorder.
 Qed.
 
 Lemma produces_silent_closed {S} `{StateType S}  S' `{StateType S'}  (σ1 σ1':S) (σ2 σ2':S')
@@ -330,245 +209,6 @@ Proof.
     eapply prefix_star2_silent; eauto.
   - eapply prefix_star2_silent'; eauto. eapply H3.
     eapply prefix_star2_silent; eauto.
-Qed.
-
-(** * Trace Equivalence (maximal traces) *)
-
-CoInductive stream (A : Type) : Type :=
-| sil : stream A
-| sons : A -> stream A -> stream A.
-
-Arguments sil [A].
-
-CoInductive coproduces {S} `{StateType S} : S -> stream extevent -> Prop :=
-| CoProducesExtern (σ σ' σ'':S) evt L :
-    star2 step σ nil σ'
-      -> activated σ'
-      -> step σ' evt σ''
-      -> coproduces σ'' L
-      -> coproduces σ (sons (EEvtExtern evt) L)
-| CoProducesSilent (σ:S) :
-    diverges σ
-    -> coproduces σ sil
-| CoProducesTerm (σ:S) (σ':S) r
-  : result σ' = r
-    -> star2 step σ nil σ'
-    -> normal2 step σ'
-    -> coproduces σ (sons (EEvtTerminate r) sil).
-
-(** ** Several closedness properties *)
-
-Lemma coproduces_reduction_closed_step S `{StateType S} (σ σ':S) L
-: coproduces σ L -> step σ EvtTau σ'  -> coproduces σ' L.
-Proof.
-  intros. inv H0.
-  - exploit activated_star_reach. eapply H3. eauto.
-    eapply (star2_step EvtTau); eauto. econstructor.
-    econstructor. eapply H6. eauto. eauto. eauto.
-  - econstructor. eapply diverges_reduction_closed; eauto.
-    eapply (star2_step EvtTau); eauto. econstructor.
-  - relsimpl.
-    econstructor; eauto.
-Qed.
-
-Lemma coproduces_reduction_closed S `{StateType S} (σ σ':S) L
-: coproduces σ L -> star2 step σ nil σ'  -> coproduces σ' L.
-Proof.
-  intros. general induction H1; eauto using coproduces. eauto.
-  destruct yl, y; simpl in *; try congruence.
-  eapply IHstar2; eauto.
-  eapply coproduces_reduction_closed_step; eauto.
-Qed.
-
-Lemma coproduces_expansion_closed_step S `{StateType S} (σ σ':S) L
-: coproduces σ' L -> step σ EvtTau σ'  -> coproduces σ L.
-Proof.
-  intros. inv H0.
-  - econstructor; eauto.
-    eapply star2_trans_silent; eauto using star2_silent, star2_refl.
-  - econstructor; eauto. econstructor; eauto.
-  - econstructor; eauto using star2_silent, star2_refl.
-Qed.
-
-
-(** ** Bisimilarity is sound for maximal traces *)
-Lemma bisim_coproduces S `{StateType S} S' `{StateType S'} (sigma:S) (σ':S')
-  : bisim sigma σ' -> forall L, coproduces sigma L -> coproduces σ' L.
-Proof.
-  revert sigma σ'. cofix COH; intros.
-  inv H2.
-  - assert (sim bot3 Bisim σ'0 σ').
-    eapply sim_reduction_closed. eapply (bisim_simp _ H1).
-    eauto. econstructor.
-    exploit (bisim_activated H4 H7). dcr.
-    edestruct H11. eauto. dcr.
-    econstructor; try eapply H10. eauto. eauto.
-    eapply COH; eauto.
-    eapply simp_bisim. eauto.
-  - econstructor. eapply (bisim_sound_diverges H1); eauto.
-  - exploit (bisim_terminate H4 H5 (bisim_simp _ H1)).
-    dcr.
-    econstructor; eauto.
-Qed.
-
-(** ** Prefix trace equivalence coincides with maximal trace equivalence. *)
-
-Lemma produces_coproduces' S `{StateType S} S' `{StateType S'} (σ:S) (σ':S')
-: (forall L, prefix σ L <-> prefix σ' L)
-  -> (forall T, coproduces σ T -> coproduces σ' T).
-Proof.
-  revert σ σ'.
-  cofix f; intros.
-  inv H2.
-  - assert (prefix σ (EEvtExtern evt::nil)).
-    eapply prefix_star_activated; eauto. econstructor 4.
-    eapply H1 in H7.
-    eapply prefix_extevent in H7. dcr.
-    econstructor. eauto. eauto. eauto. eapply f; try eapply H6.
-    eapply (prefix_preserved _ _ _ H1); eauto.
-  - exploit (produces_diverges H1 H3).
-    econstructor. eauto.
-  - assert (prefix σ (EEvtTerminate (result σ'0)::nil)).
-    econstructor 3; eauto. eapply H1 in H3.
-    eapply prefix_terminates in H3. dcr.
-    econstructor 3; eauto.
-Qed.
-
-Lemma produces_coproduces S `{StateType S} S' `{StateType S'} (σ:S) (σ':S')
-: (forall L, prefix σ L <-> prefix σ' L)
-  -> (forall T, coproduces σ T <-> coproduces σ' T).
-Proof.
-  split; eapply produces_coproduces'; eauto. symmetry; eauto.
-Qed.
-
-(** ** Bisimilarity is complete for prefix trace equivalence. *)
-
-Require Import Classical_Prop Coq.Logic.Epsilon.
-
-Lemma neither_diverges S `{StateType S} (σ:S)
-  (H0 : ~ (exists σ' : S, star2 step σ nil σ' /\ normal2 step σ'))
-  (H1 : ~ (exists σ' : S, star2 step σ nil σ' /\ activated σ'))
-  : diverges σ.
-Proof.
-  revert σ H0 H1. cofix f.
-  intros. destruct (@step_dec _ H σ).
-  - inv H2; dcr.
-    destruct x.
-    + exfalso. eapply H1; eexists σ; split; eauto using star2_refl.
-      do 2 eexists; eauto.
-    + econstructor. eauto. eapply f; intro; dcr.
-      * eapply H0; eexists; split; eauto. eapply star2_silent; eauto.
-      * eapply H1; eexists; split; eauto. eapply star2_silent; eauto.
-  - exfalso. eapply H0; eexists σ; split; eauto using star2_refl.
-Qed.
-
-Lemma three_possibilities S `{StateType S} (σ:S)
-: (exists σ', star2 step σ nil σ' /\ normal2 step σ')
-  \/ (exists σ', star2 step σ nil σ' /\ activated σ')
-  \/ diverges σ.
-Proof.
-  destruct (classic (exists σ' : S, star2 step σ nil σ' /\ normal2 step σ')); eauto; right.
-  destruct (classic (exists σ' : S, star2 step σ nil σ' /\ activated σ')); eauto; right.
-  eapply neither_diverges; eauto.
-Qed.
-
-Require Import Coq.Logic.ClassicalDescription.
-
-Lemma three_possibilities_strong S `{StateType S} (σ:S)
-: { σ' : S | star2 step σ nil σ' /\ normal2 step σ' }
-  + { σ' : S & { p : star2 step σ nil σ' &
-                     { ext : extern & { σ'' : S | step σ' (EvtExtern ext) σ'' } } } }
-  + diverges σ.
-Proof.
-  destruct (excluded_middle_informative (exists σ' : S, star2 step σ nil σ' /\ normal2 step σ')); eauto.
-  - eapply constructive_indefinite_description in e. eauto.
-  - destruct (excluded_middle_informative (exists σ' : S, star2 step σ nil σ' /\ activated σ')).
-    + eapply constructive_indefinite_description in e.
-      left; right. destruct e. eexists x; eauto. dcr; eauto.
-      eapply constructive_indefinite_description in H1. destruct H1.
-      eapply constructive_indefinite_description in e. destruct e.
-      eauto.
-    + right. revert σ n n0. cofix f.
-      intros. destruct (@step_dec _ H σ).
-      * inv H0; dcr.
-        destruct x.
-        -- exfalso. eapply n0; eexists σ; split; eauto using star2_refl.
-           do 2 eexists; eauto.
-        -- econstructor. eauto. eapply f; intro; dcr.
-           ++ eapply n; eexists; split; eauto. eapply star2_silent; eauto.
-           ++ eapply n0; eexists; split; eauto. eapply star2_silent; eauto.
-      * exfalso. eapply n; eexists σ; split; eauto using star2_refl.
-Qed.
-
-CoFixpoint tr S `{StateType S} (σ:S) : stream extevent.
-Proof.
-  destruct (three_possibilities_strong σ) as [[|]|].
-  - destruct s.
-    eapply (sons (EEvtTerminate (result x)) sil).
-  - destruct s as [? [? ?]]. destruct s. destruct s.
-    eapply (sons (EEvtExtern (EvtExtern x1)) (tr S H x2)).
-  - eapply sil.
-Defined.
-
-Definition stream_match A (s:stream A) :=
-  match s with
-  | sil => sil
-  | sons a b => sons a b
-  end.
-
-Lemma stream_id A (s:stream A)
-  : s = stream_match s.
-Proof.
-  destruct s. reflexivity. reflexivity.
-Qed.
-
-Lemma coproduces_total S `{StateType S} (σ:S)
-  : coproduces σ (tr σ).
-Proof.
-  revert σ.
-  cofix f; intros.
-  rewrite stream_id. simpl.
-  destruct (three_possibilities_strong σ) as [[|]|].
-  - destruct s. econstructor. reflexivity. eauto. eauto.
-  - destruct s. destruct s. destruct s. destruct s.
-    econstructor; eauto.
-    do 2 eexists; eauto.
-  - econstructor; eauto.
-Qed.
-
-Lemma coproduces_prefix S `{StateType S} S' `{StateType S'} (σ:S) (σ':S')
-  : (forall T, coproduces σ T -> coproduces σ' T)
-      -> forall L, prefix σ L -> prefix σ' L.
-Proof.
-  intros. general induction H2.
-  - eapply IHprefix; eauto using coproduces_expansion_closed_step.
-  - assert (coproduces σ (sons (EEvtExtern evt) (tr σ'))). {
-      econstructor 1; eauto using star2_silent, star2_refl.
-      eapply coproduces_total.
-    }
-    eapply H4 in H5. inv H5.
-    eapply prefix_star_activated; eauto.
-    eapply IHprefix.
-    intros.
-    assert (coproduces σ (sons (EEvtExtern evt) T)). {
-      econstructor 1; eauto using star2_silent, star2_refl.
-    }
-    eapply H4 in H7. inv H7.
-    relsimpl.
-    exploit (step_externally_determined _ _ _ _ H11 H17). subst. eauto.
-  - assert (coproduces σ (sons (EEvtTerminate (result σ')) sil)). {
-      econstructor; eauto.
-    }
-    eapply H4 in H0. inv H0.
-    econstructor 3; eauto.
-  - econstructor 4.
-Qed.
-
-Lemma coproduces_prefix_iff S `{StateType S} S' `{StateType S'} (σ:S) (σ':S')
-  : (forall T, coproduces σ T <-> coproduces σ' T)
-    -> forall L, prefix σ L <-> prefix σ' L.
-Proof.
-  split; eapply coproduces_prefix; firstorder.
 Qed.
 
 Lemma prefix_bisim S `{StateType S} S' `{StateType S'} (σ:S) (σ':S')
@@ -614,45 +254,4 @@ Proof.
   - assert (diverges σ').
     eapply (produces_diverges H1); eauto.
     eapply bisim_complete_diverges; eauto.
-Qed.
-
-Lemma coproduces_terminates S `{StateType S} (σ:S) r T
-:  coproduces σ (sons (EEvtTerminate r) T)
-   -> exists σ', star2 step σ nil σ' /\ normal2 step σ' /\ result σ' = r /\ T = sil.
-Proof.
-  intros. inv H0.
-  - eexists; intuition; eauto.
-Qed.
-
-Lemma diverges_coproduces_only_sil S `{StateType S} S' `{StateType S'} (σ:S)
-: diverges σ -> (forall T, coproduces σ T -> T = sil).
-Proof.
-  intros. inv H2.
-  - exfalso.
-    eapply diverges_reduction_closed in H1; eauto.
-    eapply @diverges_never_activated in H1; eauto.
-  - reflexivity.
-  - exfalso.
-    eapply diverges_reduction_closed in H1; eauto.
-    eapply @diverges_never_terminates in H1; eauto.
-Qed.
-
-Lemma coproduces_diverges S `{StateType S} S' `{StateType S'} (σ:S) (σ':S')
-: (forall L, coproduces σ L <-> coproduces σ' L)
-  -> diverges σ -> diverges σ'.
-Proof.
-  intros.
-  assert (coproduces σ sil). {
-    econstructor; eauto.
-  }
-  eapply H1 in H3.
-  inv H3. eauto.
-Qed.
-
-Lemma coproduced_bisim S `{StateType S} S' `{StateType S'} (σ:S) (σ':S')
-: (forall L, coproduces σ L <-> coproduces σ' L)
-  -> bisim σ σ'.
-Proof.
-  intros. eapply prefix_bisim.
-  eapply coproduces_prefix_iff. eauto.
 Qed.
