theories/Equiv/CoTraces.v
@@ -1,0 +1,233 @@
+Require Import List.
+Require Import Util Var Val Exp Env Map CSet AutoIndTac IL AllInRel.
+Require Import SmallStepRelations StateType StateTypeProperties.
+Require Import NonParametricBiSim Divergence TraceEquiv.
+
+Set Implicit Arguments.
+Unset Printing Records.
+
+(** * Trace Equivalence (maximal traces) *)
+
+CoInductive stream (A : Type) : Type :=
+| sil : stream A
+| sons : A -> stream A -> stream A.
+
+Arguments sil [A].
+
+CoInductive coproduces {S} `{StateType S} : S -> stream extevent -> Prop :=
+| CoProducesExtern (σ σ' σ'':S) evt L :
+    star2 step σ nil σ'
+      -> activated σ'
+      -> step σ' evt σ''
+      -> coproduces σ'' L
+      -> coproduces σ (sons (EEvtExtern evt) L)
+| CoProducesSilent (σ:S) :
+    diverges σ
+    -> coproduces σ sil
+| CoProducesTerm (σ:S) (σ':S) r
+  : result σ' = r
+    -> star2 step σ nil σ'
+    -> normal2 step σ'
+    -> coproduces σ (sons (EEvtTerminate r) sil).
+
+(** ** Several closedness properties *)
+
+Lemma coproduces_reduction_closed_step S `{StateType S} (σ σ':S) L
+: coproduces σ L -> step σ EvtTau σ'  -> coproduces σ' L.
+Proof.
+  intros. inv H0.
+  - exploit activated_star_reach. eapply H3. eauto.
+    eapply (star2_step EvtTau); eauto. econstructor.
+    econstructor. eapply H6. eauto. eauto. eauto.
+  - econstructor. eapply diverges_reduction_closed; eauto.
+    eapply (star2_step EvtTau); eauto. econstructor.
+  - relsimpl.
+    econstructor; eauto.
+Qed.
+
+Lemma coproduces_reduction_closed S `{StateType S} (σ σ':S) L
+: coproduces σ L -> star2 step σ nil σ'  -> coproduces σ' L.
+Proof.
+  intros. general induction H1; eauto using coproduces. eauto.
+  destruct yl, y; simpl in *; try congruence.
+  eapply IHstar2; eauto.
+  eapply coproduces_reduction_closed_step; eauto.
+Qed.
+
+Lemma coproduces_expansion_closed_step S `{StateType S} (σ σ':S) L
+: coproduces σ' L -> step σ EvtTau σ'  -> coproduces σ L.
+Proof.
+  intros. inv H0.
+  - econstructor; eauto.
+    eapply star2_trans_silent; eauto using star2_silent, star2_refl.
+  - econstructor; eauto. econstructor; eauto.
+  - econstructor; eauto using star2_silent, star2_refl.
+Qed.
+
+
+(** ** Bisimilarity is sound for maximal traces *)
+Lemma bisim_coproduces S `{StateType S} S' `{StateType S'} (sigma:S) (σ':S')
+  : bisim sigma σ' -> forall L, coproduces sigma L -> coproduces σ' L.
+Proof.
+  revert sigma σ'. cofix COH; intros.
+  inv H2.
+  - assert (bisim σ'0 σ'). {
+      eapply bisim_reduction_closed.
+      eauto. eauto.
+    }
+    exploit (bisim_activated H4 H7). dcr.
+    edestruct H11. eauto. dcr.
+    econstructor; try eapply H10. eauto. eauto.
+    eapply COH; eauto.
+  - econstructor. eapply (bisim_sound_diverges H1); eauto.
+  - exploit (bisim_terminate H4 H5 H1).
+    dcr.
+    econstructor; eauto.
+Qed.
+
+(** ** Prefix trace equivalence coincides with maximal trace equivalence. *)
+
+Lemma produces_coproduces' S `{StateType S} S' `{StateType S'} (σ:S) (σ':S')
+: (forall L, prefix σ L <-> prefix σ' L)
+  -> (forall T, coproduces σ T -> coproduces σ' T).
+Proof.
+  revert σ σ'.
+  cofix f; intros.
+  inv H2.
+  - assert (prefix σ (EEvtExtern evt::nil)).
+    eapply prefix_star_activated; eauto. econstructor 4.
+    eapply H1 in H7.
+    eapply prefix_extevent in H7. dcr.
+    econstructor. eauto. eauto. eauto. eapply f; try eapply H6.
+    eapply (prefix_preserved _ _ _ H1); eauto.
+  - exploit (produces_diverges H1 H3).
+    econstructor. eauto.
+  - assert (prefix σ (EEvtTerminate (result σ'0)::nil)).
+    econstructor 3; eauto. eapply H1 in H3.
+    eapply prefix_terminates in H3. dcr.
+    econstructor 3; eauto.
+Qed.
+
+Lemma produces_coproduces S `{StateType S} S' `{StateType S'} (σ:S) (σ':S')
+: (forall L, prefix σ L <-> prefix σ' L)
+  -> (forall T, coproduces σ T <-> coproduces σ' T).
+Proof.
+  split; eapply produces_coproduces'; eauto. symmetry; eauto.
+Qed.
+
+(** ** Bisimilarity is complete for prefix trace equivalence. *)
+
+Require Import Classical_Prop Coq.Logic.Epsilon.
+
+
+CoFixpoint tr S `{StateType S} (σ:S) : stream extevent.
+Proof.
+  destruct (three_possibilities_strong σ) as [[|]|].
+  - destruct s.
+    eapply (sons (EEvtTerminate (result x)) sil).
+  - destruct s as [? [? ?]]. destruct s. destruct s.
+    eapply (sons (EEvtExtern (EvtExtern x1)) (tr S H x2)).
+  - eapply sil.
+Defined.
+
+Definition stream_match A (s:stream A) :=
+  match s with
+  | sil => sil
+  | sons a b => sons a b
+  end.
+
+Lemma stream_id A (s:stream A)
+  : s = stream_match s.
+Proof.
+  destruct s. reflexivity. reflexivity.
+Qed.
+
+Lemma coproduces_total S `{StateType S} (σ:S)
+  : coproduces σ (tr σ).
+Proof.
+  revert σ.
+  cofix f; intros.
+  rewrite stream_id. simpl.
+  destruct (three_possibilities_strong σ) as [[|]|].
+  - destruct s. econstructor. reflexivity. eauto. eauto.
+  - destruct s. destruct s. destruct s. destruct s.
+    econstructor; eauto.
+    do 2 eexists; eauto.
+  - econstructor; eauto.
+Qed.
+
+Lemma coproduces_prefix S `{StateType S} S' `{StateType S'} (σ:S) (σ':S')
+  : (forall T, coproduces σ T -> coproduces σ' T)
+      -> forall L, prefix σ L -> prefix σ' L.
+Proof.
+  intros. general induction H2.
+  - eapply IHprefix; eauto using coproduces_expansion_closed_step.
+  - assert (coproduces σ (sons (EEvtExtern evt) (tr σ'))). {
+      econstructor 1; eauto using star2_silent, star2_refl.
+      eapply coproduces_total.
+    }
+    eapply H4 in H5. inv H5.
+    eapply prefix_star_activated; eauto.
+    eapply IHprefix.
+    intros.
+    assert (coproduces σ (sons (EEvtExtern evt) T)). {
+      econstructor 1; eauto using star2_silent, star2_refl.
+    }
+    eapply H4 in H7. inv H7.
+    relsimpl.
+    exploit (step_externally_determined _ _ _ _ H11 H17). subst. eauto.
+  - assert (coproduces σ (sons (EEvtTerminate (result σ')) sil)). {
+      econstructor; eauto.
+    }
+    eapply H4 in H0. inv H0.
+    econstructor 3; eauto.
+  - econstructor 4.
+Qed.
+
+Lemma coproduces_prefix_iff S `{StateType S} S' `{StateType S'} (σ:S) (σ':S')
+  : (forall T, coproduces σ T <-> coproduces σ' T)
+    -> forall L, prefix σ L <-> prefix σ' L.
+Proof.
+  split; eapply coproduces_prefix; firstorder.
+Qed.
+
+Lemma coproduces_terminates S `{StateType S} (σ:S) r T
+:  coproduces σ (sons (EEvtTerminate r) T)
+   -> exists σ', star2 step σ nil σ' /\ normal2 step σ' /\ result σ' = r /\ T = sil.
+Proof.
+  intros. inv H0.
+  - eexists; intuition; eauto.
+Qed.
+
+Lemma diverges_coproduces_only_sil S `{StateType S} S' `{StateType S'} (σ:S)
+: diverges σ -> (forall T, coproduces σ T -> T = sil).
+Proof.
+  intros. inv H2.
+  - exfalso.
+    eapply diverges_reduction_closed in H1; eauto.
+    eapply @diverges_never_activated in H1; eauto.
+  - reflexivity.
+  - exfalso.
+    eapply diverges_reduction_closed in H1; eauto.
+    eapply @diverges_never_terminates in H1; eauto.
+Qed.
+
+Lemma coproduces_diverges S `{StateType S} S' `{StateType S'} (σ:S) (σ':S')
+: (forall L, coproduces σ L <-> coproduces σ' L)
+  -> diverges σ -> diverges σ'.
+Proof.
+  intros.
+  assert (coproduces σ sil). {
+    econstructor; eauto.
+  }
+  eapply H1 in H3.
+  inv H3. eauto.
+Qed.
+
+Lemma coproduced_bisim S `{StateType S} S' `{StateType S'} (σ:S) (σ':S')
+: (forall L, coproduces σ L <-> coproduces σ' L)
+  -> bisim σ σ'.
+Proof.
+  intros. eapply prefix_bisim.
+  eapply coproduces_prefix_iff. eauto.
+Qed.
