theories/Equiv/Divergence.v
@@ -1,0 +1,82 @@
+Require Import List.
+Require Import Util Var Val Exp Env Map CSet AutoIndTac IL AllInRel.
+Require Import SmallStepRelations StateType NonParametricBiSim.
+
+Set Implicit Arguments.
+Unset Printing Records.
+
+(** * Divergence *)
+
+CoInductive diverges S `{StateType S} : S -> Prop :=
+| DivergesI σ σ'
+  : step σ EvtTau σ'
+    -> diverges σ'
+    -> diverges σ.
+
+Lemma diverges_reduction_closed S `{StateType S} (σ σ':S)
+: diverges σ -> star2 step σ nil σ'  -> diverges σ'.
+Proof.
+  intros. general induction H1; eauto using diverges.
+  invt diverges; relsimpl. eauto.
+Qed.
+
+Lemma diverges_never_activated S `{StateType S} (σ:S)
+: activated σ -> diverges σ -> False.
+Proof.
+  intros. invt diverges; relsimpl.
+Qed.
+
+Lemma diverges_never_terminates S `{StateType S} (σ:S)
+: normal2 step σ -> diverges σ -> False.
+Proof.
+  intros. invt diverges; relsimpl.
+Qed.
+
+Lemma neither_diverges S `{StateType S} (σ:S)
+  (H0 : ~ (exists σ' : S, star2 step σ nil σ' /\ normal2 step σ'))
+  (H1 : ~ (exists σ' : S, star2 step σ nil σ' /\ activated σ'))
+  : diverges σ.
+Proof.
+  revert σ H0 H1. cofix f.
+  intros. destruct (@step_dec _ H σ).
+  - inv H2; dcr.
+    destruct x.
+    + exfalso. eapply H1; eexists σ; split; eauto using star2_refl.
+      do 2 eexists; eauto.
+    + econstructor. eauto. eapply f; intro; dcr.
+      * eapply H0; eexists; split; eauto. eapply star2_silent; eauto.
+      * eapply H1; eexists; split; eauto. eapply star2_silent; eauto.
+  - exfalso. eapply H0; eexists σ; split; eauto using star2_refl.
+Qed.
+
+
+(** ** Bisimilarity preserves silent divergence *)
+
+Lemma bisim_sound_diverges S `{StateType S} S' `{StateType S'} (σ:S) (σ':S')
+: bisim σ σ' -> diverges σ -> diverges σ'.
+Proof.
+  revert σ σ'. cofix COH; intros.
+  inv H1.
+  - eapply plus2_destr_nil in H4. dcr.
+    econstructor. eauto.
+    eapply COH; eauto.
+    eapply bisim_reduction_closed_both; try eapply H1;
+      eauto using star2_refl, star2_silent.
+  - eapply diverges_reduction_closed in H3.
+    + exfalso. eapply (diverges_never_activated H5); eauto.
+    + eapply H2.
+  - eapply diverges_reduction_closed in H4.
+    + exfalso. eapply (diverges_never_terminates H6); eauto.
+    + eapply H2.
+Qed.
+
+(** ** Silently diverging programs are bisimlar *)
+
+Lemma bisim_complete_diverges S `{StateType S} S' `{StateType S'} (σ:S) (σ':S')
+: diverges σ -> diverges σ' -> bisim σ σ'.
+Proof.
+  revert σ σ'. cofix COH; intros.
+  inv H1; inv H2.
+  econstructor. econstructor; eauto. econstructor; eauto.
+  eapply COH; eauto.
+Qed.
