theories/Equiv/StateTypeProperties.v
@@ -1,0 +1,41 @@
+Require Import StateType SmallStepRelations Divergence.
+Require Import Classical_Prop Coq.Logic.Epsilon.
+Set Implicit Arguments.
+
+Lemma three_possibilities S `{StateType S} (σ:S)
+: (exists σ', star2 step σ nil σ' /\ normal2 step σ')
+  \/ (exists σ', star2 step σ nil σ' /\ activated σ')
+  \/ diverges σ.
+Proof.
+  destruct (classic (exists σ' : S, star2 step σ nil σ' /\ normal2 step σ')); eauto; right.
+  destruct (classic (exists σ' : S, star2 step σ nil σ' /\ activated σ')); eauto; right.
+  eapply neither_diverges; eauto.
+Qed.
+
+Require Import Coq.Logic.ClassicalDescription.
+
+Lemma three_possibilities_strong S `{StateType S} (σ:S)
+: { σ' : S | star2 step σ nil σ' /\ normal2 step σ' }
+  + { σ' : S & { p : star2 step σ nil σ' &
+                     { ext : extern & { σ'' : S | step σ' (EvtExtern ext) σ'' } } } }
+  + diverges σ.
+Proof.
+  destruct (excluded_middle_informative (exists σ' : S, star2 step σ nil σ' /\ normal2 step σ')); eauto.
+  - eapply constructive_indefinite_description in e. eauto.
+  - destruct (excluded_middle_informative (exists σ' : S, star2 step σ nil σ' /\ activated σ')).
+    + eapply constructive_indefinite_description in e.
+      left; right. destruct e. eexists x; eauto. dcr; eauto.
+      eapply constructive_indefinite_description in H1. destruct H1.
+      eapply constructive_indefinite_description in e. destruct e.
+      eauto.
+    + right. revert σ n n0. cofix f.
+      intros. destruct (@step_dec _ H σ).
+      * inv H0; dcr.
+        destruct x.
+        -- exfalso. eapply n0; eexists σ; split; eauto using star2_refl.
+           do 2 eexists; eauto.
+        -- econstructor. eauto. eapply f; intro; dcr.
+           ++ eapply n; eexists; split; eauto. eapply star2_silent; eauto.
+           ++ eapply n0; eexists; split; eauto. eapply star2_silent; eauto.
+      * exfalso. eapply n; eexists σ; split; eauto using star2_refl.
+Qed.
